\documentclass[12pt, letterpaper]{article}
\usepackage{amsmath}

\begin{document}

\subsection*{Convergence of $\frac{F_{n-2}}{F_n}$}
\begin{align*}
    \frac{F_{n-2}}{F_n} &= \frac{F_{n-2}}{F_{n-2}+F_{n-1}}\\
                        &= \left(\frac{F_{n-2}}{F_{n-2}}\right)\frac{1}{1+\frac{F_{n-1}}{F_{n-2}}}\\
                        &= \frac{1}{1+\frac{F_{n-2}+F_{n-3}}{F_{n-2}}}\\
                        &= \frac{1}{2+\frac{F_{n-3}}{F_{n-2}}}\\
                        &= \frac{1}{2+\frac{1}{1+\frac{F_{n-4}}{F_{n-3}}}}\\
                        &= \ldots
\end{align*}

Clearly there is a continued fraction of the form

\begin{equation*}
    \frac{F_{n-(k+1)}}{F_{n-k}} = \frac{1}{1+\frac{F_{n-(k+2)}}{F_{n-(k+1)}}}
\end{equation*}

which expands to

\begin{equation*}
    \frac{1}{1+\frac{1}{1+\ldots}}
\end{equation*}

(TODO) which converges to $1-\phi$.

For a large enough $n$

\begin{align*}
    \frac{1}{2+\frac{F_{n-3}}{F_{n-2}}} &= \frac{1}{2+(\phi-1)}\\
                                        &= \frac{1}{1+\phi}
\end{align*}

\newpage

\subsection*{Given $n=F_i$, estimate $i$}

Given the above convergence, $F_n$ can be computed from $F_{n-2}$:

\begin{align*}
    \frac{F_{n-2}}{F_n} &= \frac{1}{1+\phi}\\
    F_n &= \left(1+\phi\right)F_{n-2}
\end{align*}

Therefore, starting from $F_1$ any $F_{2k+1}$ can be reached\footnote{Requires $k>40$, give or take.} 
by performing $(1+\phi)^{k}F_1$, $k\geq 0$.

So to find the number of steps from some $n=F_{2k+1}$ to $F_1$, solve for $k$:

\begin{align*}
    n\left(\frac{1}{1+\phi}\right)^k &= 1\\
    k &= \frac{\log\left(\frac{1}{n}\right)}{\log\left(\frac{1}{1+\phi}\right)}
\end{align*}

To get the actual index perform $2*f(n)$ as $f(n)$ skips half the indices.

TODO: Verify indices are correct, assuming $F_1 = 1, F_2=1$.

\end{document}
